lx_confl.v
@@ -1,0 +1,23 @@
+Require Import lambda_x.
+
+Fixpoint B (t : n_sexp) := match t with
+                           | n_var x => n_var x
+                           | n_abs x t1 => n_abs x (B t1)
+                           | n_app t1 t2 => match t1 with
+                                            | n_abs x t3 => m_subst (B t2) x (B t3)
+                                            | _ => n_app (B t1) (B t2)
+                                            end
+                           | n_sub t1 x t2 => n_sub (B t1) x (B t2)
+                           end.
+
+Fixpoint P (t : n_sexp) := match t with
+                           | n_var x => n_var x
+                           | n_abs x t1 => n_abs x (P t1)
+                           | n_app t1 t2 => n_app (P t1) (P t2)
+                           | n_sub t1 x t2 => m_subst (P t2) x (P t1)
+                           end.
+
+Lemma pi_P: forall t1 t2, step pix t1 t2 -> P t1 = P t2.
+Proof.
+  intros t1 t2 H. induction H.
+  - inversion H. 
